\documentclass{article}
\usepackage[T2A]{fontenc}
\usepackage[cp1251]{inputenc}
\usepackage[russian]{babel}

\begin{document}
    \begin{center}
        
        \section{}
            \[\int x(x + 1)(x - 2)dx = \int x(x^2 - x - 2)dx =
            \int (x^3 - x^2 - 2x)dx = \frac{x^4}{4} - \frac{x^3}{3} - x^2 + C\]

        \section{}
            \[\int \frac{x^2-x+1}{\sqrt{x}}dx = \int \frac{x^2}{\sqrt{x}}dx -
            \int \frac{x}{\sqrt{x}}dx + \int \frac{dx}{\sqrt{x}} =
            \int x^{\frac{3}{2}}dx - \int x^{\frac{1}{2}}dx +
            \int x^{-\frac{1}{2}}dx = \] 
            \[= \frac{2x^2 \sqrt{x}}{5} - \frac{2x \sqrt{x}}{3} + 2 \sqrt{x} + C\]    
    
        \section{}
            \[\int \sqrt{x \sqrt{x \sqrt{x}}}dx = \int x^{\frac{7}{8}}dx =
            \frac{8}{15} x^{\frac{15}{8}} + C\]
            
        \section{}
            \[\int \frac{dx}{7 + x^2} = \frac{1}{\sqrt{7}}
            \arctan{\frac{x}{\sqrt{7}}} + C\]
            
        \section{}
            \[\int \frac{dx}{2x^2 + 3} = \frac{1}{2} \int
            \frac{dx}{x^2 + \frac{3}{2}} = \frac{1}{2} \sqrt{\frac{2}{3}}
            \arctan{\left(\sqrt{\frac{2}{3}}x\right)} + C\]
            
        \section{}
            \[\int \frac{dx}{3x^2 - 7} = - \frac{1}{3}
            \int \frac{dx}{\frac{7}{3} - x^2} = - \frac{1}{3}
            \frac{1}{2 \sqrt{\frac{7}{3}}} \ln{\left|
            \frac{\sqrt{\frac{7}{3}} + x}{\sqrt{\frac{7}{3}} - x} \right|} + C\]    
    
        \section{}
            \[\int \frac{x^2}{1 - x^2}dx = \int \left(\frac{1}{1-x^2} - 1
            \right)dx = \int \frac{dx}{1 - x^2} - \int dx = 
            \frac{1}{2} \ln{\left| \frac{1 + x}{1 - x} \right|} - x + C\]

        \section{}
            \[\int \frac{dx}{x^4 - 1} = \int \left(\frac{1}{2x^2 - 2}
            - \frac{1}{2x^2 + 2}\right)dx = - \frac{1}{2} \int \frac{dx}{1 - x^2}
            - \frac{1}{2} \int \frac{dx}{x^2 + 1} =\] 
            \[= - \frac{1}{4} \ln{\left| \frac{1 + x}{1 - x} \right|} -
            \frac{1}{2} \arctan{x} + C\]

        \section{}
            \[\int \frac{(1 + x)^2}{x(1 + x^2)}dx = \int 
            \frac{x^2 + 2x + 1}{x(1 + x^2)}dx = \int \frac{x}{1 + x^2}dx
            + 2 \int \frac{dx}{1 + x^2} + \int \frac{dx}{x(1 + x^2)} =\]
            \[= \left| \frac{1}{x(1 + x^2)} = \frac{1}{x} - \frac{x}{1 + x^2}
            \right| = \int \frac{x}{1 + x^2}dx + 2 \int \frac{dx}{1 + x^2} +
            \int \frac{dx}{x} - \int \frac{x}{1 + x^2}dx =\]
            \[= \frac{1}{2} \ln{|1 + x^2|} + 2 \arctan{x} + \ln{|x|}
            - \frac{1}{2} \ln{|1 + x^2|} + C = 2 \arctan{x} + \ln{|x|} + C\]

        \section{}
            \[\int \frac{dx}{\sqrt{2 - x^2}} = \arcsin{\frac{x}{\sqrt{2}} + C}\]
            
        \section{}
            \[\int (5^x - 2^x)^2 dx = \int (5^{2x} - 2 * 10^x + 4^x)dx =
            \int 25^x dx - 2 \int 10^x dx + \int 4^x dx = \] 
            \[= \frac{25^x}{\ln{25}} - \frac{2 * 10^x}{\ln{10}} + 
            \frac{4^x}{\ln{4}} + C\]    

        \section{}
            \[\int \frac{2^x 3^{2x} 4^{3x}}{5^x 6^{2x}}dx = \int
            \left(\frac{32}{5}\right)^x dx = \left(\frac{32}{5}\right)^x
            \frac{1}{\ln{\left(\frac{32}{5}\right)}} + C\]
            
        \section{}
            \[\int \frac{e^{3x} - 1}{e^x - 1}dx =
            \int \frac{(e^x - 1)(e^{2x} + e^x + 1)}{e^x - 1}dx
            = \int e^{2x}dx + \int e^x dx + \int dx = 
            \frac{1}{2} e^{2x} + e^x + x + C\]
            
        \section{}
            \[\int \sin{\frac{x}{2}}^2 dx = \int \frac{1 - \cos{x}}{2}dx =
            \frac{1}{2} \int dx - \frac{1}{2} \int \cos{x}dx =
            \frac{x - \sin{x}}{2} + C\]      

        \end{center}
\end{document}