\section{}
    \[\int \left(\cos{\frac{x}{2}}\right)^2 dx = \int \frac{1 + \cos{x}}{2}dx =
    \frac{1}{2} \int dx + \frac{1}{2} \int \cos{x}dx = \frac{x}{2} +
    \frac{\sin{x}}{2} + C\]

\section{}
    \[\int \frac{dx}{(\sin{x})^2 (\cos{x})^2} = 4 \int \frac{dx}{(\sin{2x})^2}
    = \left| t = 2x dt = 2dx \right| = 2 \int \frac{dt}{(\sin{t})^2} =\]
    \[-2 \ctg{t} + C = -2 \ctg{2x} + C\]    

\section{}
    \[\int (\tg{x})^2 dx = \left| (\tg{x})^2 = \frac{(\sin{x})^2}{(\cos{x})^2}
    = \frac{1 - (\cos{x})^2}{(\cos{x})^2}  = 
    \frac{1}{(\cos{x})^2} - 1\right| = \]
    \[= \int \frac{dx}{(\cos{x})^2} - \int dx = \tg{x} - x + C\]

\section{}
    \[\int (\ctg{x})^2 dx = \left| (\ctg{x})^2 = 
    \frac{(\cos{x})^2}{(\sin{x})^2} = \frac{1 - (\sin{x})^2}{(\sin{x})^2} = 
    \frac{1}{(\sin{x})^2} - 1 \right| = \]
    \[= \int \frac{dx}{(\sin{x})^2} - \int dx = - \ctg{x} - x + C\]
    
\section{}
    \[\int \frac{dx}{2x + 3} = \left| 2x + 3 = t, \quad dt = 2dx \right| =
    \frac{1}{2} \int \frac{dt}{t} = \frac{1}{2} \ln{|t|} + C =
    \frac{1}{2} \ln|2x + 3| + C\]
    
\section{}
    \[\int \frac{x + 3}{(x + 2)(x - 1)}dx = \left| t = x - 1, \quad dt = dx
    \right| = \int \frac{t + 4}{t(t + 3)}dt =\]
    \[= \int \frac{dt}{t + 3} + 4 \int \frac{dt}{t(t + 3)} = 
    \int \frac{dt}{t + 3} + \frac{4}{3}(\int \frac{dt}{t} - \int \frac{dt}{t + 3}) =\]
    \[= \left|t + 3 = q, \quad dq = dt \right| = \int \frac{dq}{q} +
    \frac{4}{3} \int \frac{dt}{t} - \frac{4}{3} \int \frac{dq}{q} =\]
    \[= -\frac{1}{3} \ln{|q|} + \frac{4}{3} \ln{|t|} + C =
    -\frac{1}{3} \ln{|x + 2|} + \frac{4}{3} \ln{|x - 1|} + C\]
    
\section{}
    \[\int \frac{2 + x}{1 + x}dx = \int (\frac{1}{1 + x} + 1)dx =
    \int \frac{dx}{1 + x} + \int dx = \left|1 + x = t, \quad dt = dx \right| =\]
    \[= \int \frac{dt}{t} + \int dx = \ln{|t|} + x + C = \ln{|1 + x|} + x + C\]

\section{}
    \[\int (2x + 5)^{15} dx = \left|t = 2x + 5, \quad dt = 2dx \right| =
    \frac{1}{2} \int t^{15} dt = \frac{t^{16}}{32} + C =\]
    \[= \frac{(2x + 5)^{16}}{32} + C\]    

\section{}
    \[\int x(x - 2)^5 dx = \left|t = x - 2, \quad x = t + 2, \quad dt = dx
    \right| = \int (t + 2)t^5 dt = \int (t^6 + 2t^5)dt =\]
    \[= \int t^6 dt + 2 \int t^5 dt = \frac{t^7}{7} + \frac{t^6}{3} + C =
    \frac{(x - 2)^7}{7} + \frac{(x - 2)^6}{3} + C\]
    
\section{}
    \[\int (x + 2)\sqrt{x - 2}dx \left|t = x - 2, \quad x + 2 = t + 4,
    \quad dt = dx \right| = \int (t + 4)\sqrt{t}dt =\]
    \[= \int t^{\frac{3}{2}}dt + 4 \int t^{\frac{1}{2}}dt =
    \frac{2}{5} t^{\frac{5}{2}} + \frac{8}{3} t^{\frac{3}{2}} + C =
    \frac{2(x - 2)^{\frac{5}{2}}}{5} + \frac{8(x - 2)^{\frac{3}{2}}}{2} + C\]  
    
\section{}
    \[\int \frac{2x - 7}{\sqrt{1 + 3x}}dx = \left|t = 1 + 3x, \quad dt = 3dx,
    \quad 2x - 7 = \frac{2t - 23}{3}, \quad x = \frac{t - 1}{3} \right| =\]
    \[= \frac{1}{9} \int \frac{2t - 23}{\sqrt{t}}dt =
    \frac{2}{9} \int t^{\frac{1}{2}}dt - \frac{23}{9} \int t^{-\frac{1}{2}}dt 
    = \frac{4}{27} (1 + 3x)^{\frac{3}{2}} - \frac{46}{9} \sqrt{1 + 3x} + C\]

\section{}
    \[\int \frac{x^2 + 1}{2x - 1} dx = \left|t = 2x - 1, \quad dt = 2dx,
    \quad x = \frac{t + 1}{2} \right| = \frac{1}{4} (\int tdt + 2 \int dt +
    5 \int dt) =\] 
    \[= \frac{1}{4} (\frac{t^2}{2} + 2t + 5t) + C = 
    \frac{t^2}{8} + \frac{t}{2} + \frac{5t}{4} + C =
    \frac{(2x - 1)^2}{8} + \frac{2x - 1}{2} + \frac{2(2x - 1)}{4} + C\]
    
\section{}
    \[\int (2x + 3)^2 (1 - x)^8 dx = \left|t = 1 - x, \quad dt = -dx,
    \quad x = 1 - t, \quad 2x + 3 = -2t + 5 \right| =\]
    \[- \int (-2t + 5)^2 t^8 dt = - \int (4t^2 - 20t + 25)t^8 dt = 
    -4 \int t^{10} dt + 20 \int t^9 dt - 25 \int t^8 dt =\]
    \[= - \frac{4 t^{11}}{11} + 2 t^{10} - \frac{25 t^9}{9} + C =
    - \frac{4 (1 - x)^{11}}{11} + 2(1 - x)^{10} - \frac{25 (1 - x)^9}{9} + C\]
    
\section{}
    \[\int \frac{x - 4}{\sqrt{x^2 - 2}}dx = \int \frac{x}{\sqrt{x^2 -2}}dx
    - 4 \int \frac{dx}{\sqrt{x^2 - 2}} =\]
    \[= \left|t = x^2 - 2, \quad dt = 2xdx \right| = 
    \frac{1}{2} \int \frac{dt}{\sqrt{t}} - 4 \int \frac{dx}{\sqrt{x^2 - 2}} =
    \sqrt{t} - 4 \ln|x + \sqrt{x^2- 2}| + C = \]
    \[= \sqrt{x^2 - 2} - 4 \ln{|x + \sqrt{x^2 - 2}}| + C\]    